crypto/Hacl.Box.fst
@@ -6,6 +6,7 @@ open FStar.ST
 open Hacl.Constants
 open Hacl.SecretBox
 
+
 (* Module abbreviations *)
 module HS  = FStar.HyperStack
 module B   = FStar.Buffer
@@ -14,45 +15,23 @@ module U32 = FStar.UInt32
 module U64 = FStar.UInt64
 
 
-
-val crypto_box_easy:
-  c:uint8_p ->
-  m:uint8_p ->
-  mlen:u64{let len = U64.v mlen in length c = len + crypto_box_MACBYTES /\ len = length m}  ->
-  n:uint8_p{length n = crypto_box_NONCEBYTES} ->
-  pk:uint8_p{length pk = crypto_box_PUBLICKEYBYTES} ->
-  sk:uint8_p{length sk = crypto_box_SECRETKEYBYTES} ->
+val crypto_box_beforenm:
+  k:uint8_p{length k = crypto_box_PUBLICKEYBYTES} ->
+  pk:uint8_p{length pk = crypto_box_PUBLICKEYBYTES /\ disjoint k pk} ->
+  sk:uint8_p{length sk = crypto_box_SECRETKEYBYTES /\ disjoint k sk} ->
   Stack u32
-    (requires (fun h -> live h c /\ live h m /\ live h n /\ live h pk /\ live h sk))
-    (ensures  (fun h0 z h1 -> modifies_1 c h0 h1 /\ live h1 c))
-let crypto_box_easy c m mlen n pk sk =
+    (requires (fun h -> live h k /\ live h pk /\ live h sk))
+    (ensures  (fun h0 _ h1 -> modifies_1 k h0 h1))
+let crypto_box_beforenm k pk sk =
   push_frame();
-  let key = create (Hacl.Cast.uint8_to_sint8 0uy) 32ul in
+  let tmp = create (Hacl.Cast.uint8_to_sint8 0uy) 48ul in
+  let hsalsa_k = sub tmp 0ul 32ul in
+  let hsalsa_n = sub tmp 32ul 16ul in
   (* Compute shared key *)
-  Hacl.EC.Curve25519.exp key pk sk;
-  let z = crypto_secretbox_easy c m mlen n key in
+  Hacl.EC.Curve25519.exp hsalsa_k pk sk;
+  Hacl.Symmetric.HSalsa20.crypto_core_hsalsa20 k hsalsa_n hsalsa_k;
   pop_frame();
-  z
-
-
-val crypto_box_open_easy:
-  m:uint8_p ->
-  c:uint8_p ->
-  mlen:u64{let len = U64.v mlen in length m = len - crypto_box_MACBYTES /\ len = length c}  ->
-  n:uint8_p{length n = crypto_box_NONCEBYTES} ->
-  pk:uint8_p{length pk = crypto_box_PUBLICKEYBYTES} ->
-  sk:uint8_p{length sk = crypto_box_SECRETKEYBYTES} ->
-  Stack u32
-    (requires (fun h -> live h c /\ live h m /\ live h n /\ live h pk /\ live h sk))
-    (ensures  (fun h0 z h1 -> modifies_1 c h0 h1 /\ live h1 c))
-let crypto_box_open_easy m c mlen n pk sk =
-  push_frame();
-  let key = create (Hacl.Cast.uint8_to_sint8 0uy) 32ul in
-  (* Compute shared key *)
-  Hacl.EC.Curve25519.exp key pk sk;
-  let z = crypto_secretbox_open_easy m c mlen n key in
-  pop_frame();
-  z
+  0ul
 
 
 val crypto_box_detached:
@@ -74,7 +53,7 @@ let crypto_box_detached c mac m mlen n pk sk =
   let hsalsa_n = sub key 64ul 16ul in
   (* Compute shared key *)
   Hacl.EC.Curve25519.exp k pk sk;
-  Hacl.Symmetric.XSalsa20.hsalsa_init subkey k hsalsa_n;
+  Hacl.Symmetric.HSalsa20.crypto_core_hsalsa20 subkey hsalsa_n k;
   let z = crypto_secretbox_detached c mac m mlen n subkey in
   pop_frame();
   z
@@ -99,7 +78,35 @@ let crypto_box_open_detached m c mac mlen n pk sk =
   let hsalsa_n = sub key 64ul 16ul in
   (* Compute shared key *)
   Hacl.EC.Curve25519.exp k pk sk;
-  Hacl.Symmetric.XSalsa20.hsalsa_init subkey k hsalsa_n;
+  Hacl.Symmetric.HSalsa20.crypto_core_hsalsa20 subkey hsalsa_n k;
   let z = crypto_secretbox_open_detached m c mac mlen n subkey in
   pop_frame();
   z
+
+
+val crypto_box_easy:
+  c:uint8_p ->
+  m:uint8_p ->
+  mlen:u64{let len = U64.v mlen in length c = len + crypto_box_MACBYTES /\ len = length m}  ->
+  n:uint8_p{length n = crypto_box_NONCEBYTES} ->
+  pk:uint8_p{length pk = crypto_box_PUBLICKEYBYTES} ->
+  sk:uint8_p{length sk = crypto_box_SECRETKEYBYTES} ->
+  Stack u32
+    (requires (fun h -> live h c /\ live h m /\ live h n /\ live h pk /\ live h sk))
+    (ensures  (fun h0 z h1 -> modifies_1 c h0 h1 /\ live h1 c))
+let crypto_box_easy c m mlen n pk sk =
+  crypto_box_detached (offset c 16ul) c m mlen n pk sk
+
+
+val crypto_box_open_easy:
+  m:uint8_p ->
+  c:uint8_p ->
+  mlen:u64{let len = U64.v mlen in length m = len - crypto_box_MACBYTES /\ len = length c}  ->
+  n:uint8_p{length n = crypto_box_NONCEBYTES} ->
+  pk:uint8_p{length pk = crypto_box_PUBLICKEYBYTES} ->
+  sk:uint8_p{length sk = crypto_box_SECRETKEYBYTES} ->
+  Stack u32
+    (requires (fun h -> live h c /\ live h m /\ live h n /\ live h pk /\ live h sk))
+    (ensures  (fun h0 z h1 -> modifies_1 c h0 h1 /\ live h1 c))
+let crypto_box_open_easy m c mlen n pk sk =
+  crypto_box_open_detached m (offset c 16ul) c (U64 (mlen -^ 16uL)) n pk sk
